work on typing

theories/prob_eff_lang/probblaze/pure_weakestpre.v
@@ -3,66 +3,194 @@ From iris.proofmode Require Import base proofmode.
 From clutch.prob_eff_lang.probblaze Require Import syntax semantics notation class_instances logic.
 
 (* Consider generalizing the PureExec construction *)
-Definition prel `{Σ : gFunctors} (e1 e2 : expr) (Φ : val → val → iProp Σ) : iProp Σ := 
-  match (to_val e1), (to_val e2) with
-  | Some v1, Some v2 => Φ v1 v2
-  | Some v1, None => ∃ (v2 : val), (∃ n2, ⌜nsteps pure_step n2 e2 v2⌝) ∗ Φ v1 v2
-  | None, Some v2 =>  ∃ (v1 : val), (∃ n1, ⌜nsteps pure_step n1 e1 v1⌝) ∗ Φ v1 v2
-  | None, None => ∃ (v1 v2 : val) n1 n2,  ⌜nsteps pure_step n1 e1 v1 ∧ nsteps pure_step n2 e2 v2⌝ ∗ Φ v1 v2
-  end. 
+(* Definition prel `{Σ : gFunctors} (e1 e2 : expr) (Φ : val → val → iProp Σ) : iProp Σ := 
+       ∃ (v1 v2 : val),
+       ⌜rtc pure_step e1 v1⌝ ∗ ⌜rtc pure_step e2 v2⌝ ∗ Φ v1 v2. *)
+  (* match (to_val e1), (to_val e2) with
+     | Some v1, Some v2 => Φ v1 v2
+     | Some v1, None => ∃ (v2 : val), (∃ n2, ⌜nsteps pure_step n2 e2 v2⌝) ∗ Φ v1 v2
+     | None, Some v2 =>  ∃ (v1 : val), (∃ n1, ⌜nsteps pure_step n1 e1 v1⌝) ∗ Φ v1 v2
+     | None, None => ∃ (v1 v2 : val) n1 n2,  ⌜nsteps pure_step n1 e1 v1 ∧ nsteps pure_step n2 e2 v2⌝ ∗ Φ v1 v2
+     end.  *)
 
-Lemma prel_intuitionistically `{Σ : gFunctors} e1 e2 Φ : 
-  (□ prel e1 e2 Φ) -∗ @prel Σ e1 e2 (λ v1 v2, □ (Φ v1 v2)).
+Definition prel_pre `{Σ : gFunctors} (Φ : val → val → iProp Σ)
+    (R : (expr * expr) -d> iProp Σ) : (expr * expr) -d> iProp Σ :=
+  λ ee, let (e1, e2) := ee in
+  match to_val e1, to_val e2 with
+  | Some v1, Some v2 => Φ v1 v2
+  | Some v1, None    => (∀ e2', ⌜pure_step e2 e2'⌝ -∗ R ((Val v1), e2'))%I
+  | None,    Some v2 => (∀ e1', ⌜pure_step e1 e1'⌝ -∗ R (e1', (Val v2)))%I
+  | None,    None    => (∀ e1', ⌜pure_step e1 e1'⌝ -∗ R (e1', e2))%I
+  end.
+
+Local Lemma prel_pre_mono `{Σ : gFunctors} (wp1 wp2 : expr * expr → iProp Σ) Φ :
+  ⊢ (□ ∀ ee, wp1 ee -∗ wp2 ee) →
+    ∀ ee, prel_pre Φ wp1 ee -∗ prel_pre Φ wp2 ee.
 Proof.
-  iIntros "#Hrel". unfold prel.
-  destruct (to_val e1) eqn:Heq1, (to_val e2) eqn:Heq2; first done.
-  1, 2: iDestruct "Hrel" as (??) "H"; iExists _; iSplit; first (by iPureIntro); by iModIntro. 
-  iDestruct "Hrel" as (????) "H". iExists _,_,_,_. iDestruct "H" as "($ & H2)". by iModIntro. 
+  iIntros "#H"; iIntros ((e1, e2)) "Hwp". rewrite /prel_pre.
+  destruct (to_val e1), (to_val e2) as [v1 v2|]; first done; iIntros (e') "He'"; iApply "H"; by iApply "Hwp".
 Qed.
+
+Local Instance prel_pre_mono_pred `{Σ : gFunctors } Φ :
+  BiMonoPred (@prel_pre Σ Φ).
+Proof.
+  constructor; last solve_proper.
+  iIntros (wp1 wp2 ??) "#H". by iApply prel_pre_mono.
+Qed.
+
+Local Definition prel_def `{!probblazeRGS Σ}
+    (e1 e2 : expr) (Φ : val → val → iProp Σ) : iProp Σ :=
+  bi_least_fixpoint (prel_pre Φ) (e1, e2).
+Local Definition prel_aux : seal (@prel_def). Proof. by eexists. Qed.
+Definition prel := prel_aux.(unseal).
+Global Arguments prel {Σ _}.
+Local Lemma prel_unseal `{!probblazeRGS Σ} : prel = @prel_def Σ _.
+Proof. rewrite -prel_aux.(seal_eq) //. Qed.
 
 Notation "'PREL' e1 ≤ e2 '[{' Φ '}]'" := (prel e1%E e2%E Φ)
                                            (at level 20, e1, e2, Φ at next level, only parsing) : bi_scope.
 Notation "'PREL' e1 ≤ e2 '[{' v1 ; v2 , Φ '}]'" := (prel e1%E e2%E (λ v1 v2, Φ)%I)
                                                    (at level 20, v1 ident, v2 ident, e1, e2, Φ at next level) : bi_scope.
 
+Section prel.
+  Context `{!probblazeRGS Σ}.
 
-Lemma prel_brel `{!probblazeRGS Σ} e1 e2 Φ :                         
+Lemma prel_unfold e1 e2 Φ :
+  prel e1 e2 Φ ⊣⊢ prel_pre Φ (fun '(e1', e2') => prel e1' e2' Φ) (e1, e2).
+Proof. by rewrite prel_unseal /prel /prel_def least_fixpoint_unfold. Qed.
+Lemma prel_ind Φ `{NonExpansive Ψ} :
+  □ (∀ e, prel_pre Φ (λ '(e1, e2), Ψ (e1, e2) ∧ PREL e1 ≤ e2 [{ v1; v2, Φ v1 v2 }]) e -∗ Ψ e) -∗
+  (∀ e1 e2, PREL e1 ≤ e2 [{ v1; v2, Φ v1 v2 }] -∗ Ψ (e1, e2)). 
+Proof.
+  iIntros "#IH" (e1 e2) "H //=". rewrite prel_unseal.
+  iApply (least_fixpoint_ind _ Ψ with "IH H").
+Qed.
+
+Lemma prel_intuitionistically e1 e2 Φ : 
+  (□ prel e1 e2 Φ) -∗ prel e1 e2 (λ v1 v2, □ (Φ v1 v2)).
+Proof.
+  iIntros "#H". iAssert (PREL e1 ≤ e2 [{ v1; v2, Φ v1 v2 }])%I as "H'"; first done.
+  iRevert "H H'". rewrite {1}bi.intuitionistically_elim. iRevert (e1 e2).
+  iApply (@prel_ind _ (λ ee, □ PREL ee.1 ≤ ee.2 [{v1; v2, Φ v1 v2}] -∗ PREL ee.1 ≤ ee.2 [{v1; v2, (□ Φ v1 v2)}])%I).
+  1 : solve_proper.
+  iIntros ((e1, e2)) "!# IH #H //=".
+  rewrite !prel_unfold /prel_pre.
+  destruct (to_val e1) as [v1|]; destruct (to_val e2) as [v2|]; first done.
+  all : iIntros (?) "#Hs"; iApply ("IH" with "[$]"); iModIntro; by iApply "H".
+Qed. 
+
+Notation "'PREL' e1 ≤ e2 '[{' Φ '}]'" := (prel e1%E e2%E Φ)
+                                           (at level 20, e1, e2, Φ at next level, only parsing) : bi_scope.
+Notation "'PREL' e1 ≤ e2 '[{' v1 ; v2 , Φ '}]'" := (prel e1%E e2%E (λ v1 v2, Φ)%I)
+                                                   (at level 20, v1 ident, v2 ident, e1, e2, Φ at next level) : bi_scope.
+Lemma pure_step_eq (e : expr) e1 e2 : pure_step e e1 → pure_step e e2 → e1 = e2.
+Proof.
+  intros He1 He2.
+  inversion He1. inversion He2.
+  simpl in *.
+  eapply det_step_is_unique.
+Admitted.
+
+
+Lemma brel_step_r e1 e2 Φ :
+  (∀ e2', ⌜pure_step e2 e2'⌝ -∗ brel ⊤ e1 e2' ⊥ Φ) -∗ brel ⊤ e1 e2 ⊥ Φ.
+Proof.
+  iIntros "Hstep".
+  
+Admitted.
+
+Lemma prel_brel e1 e2 Φ :                         
   prel e1 e2 Φ -∗ brel ⊤ e1 e2 ⊥ Φ.
 Proof. 
-(*   iIntros "He". 
-     destruct (to_val e1) eqn:Heq1, (to_val e2) eqn:Heq2; rewrite /prel Heq1 Heq2/=.
-     - rewrite -(of_to_val _ _ Heq1). rewrite -(of_to_val _ _ Heq2). iApply brel_value. by iIntros "$ !>".
-     - rewrite -(of_to_val _ _ Heq1). iDestruct "He" as (???) "HΦ".
-       iApply brel_pure_step_r; [intros ?; done|done| ].
+  iRevert (e1 e2).
+  iApply (@prel_ind _ (λ e, brel ⊤ e.1 e.2 ⊥ Φ)).
+  1 : solve_proper.
+  iIntros ((e1,e2)) "!# IH //=".
+  destruct (to_val e1) as [v1|] eqn:He1; destruct (to_val e2) as [v2|] eqn:He2.
+  - apply of_to_val in He1 as <-. apply of_to_val in He2 as <-.
+    iApply brel_value. by iIntros "$ !>".
+  - apply of_to_val in He1 as <-. iApply brel_step_r. iIntros (?) "Hs". 
+    iDestruct ("IH" with "Hs") as "($&_)".
+    
+  (* provable *)
+  (* iIntros "(%&%&%He1&%He2&HΦ)". 
+     apply rtc_nsteps in He1 as (n&He1).
+     apply rtc_nsteps in He2 as (m&He2).
+     destruct n, m. 
+     - inversion He1. inversion He2. simplify_eq.
        iApply brel_value. by iIntros "$ !>".
-     - rewrite -(of_to_val _ _ Heq2). iDestruct "He" as (???) "HΦ".
-       iApply brel_pure_step_later; [intros ?; done|done|]. iApply brel_value. by iIntros "!> $ !>".
-     - iDestruct "He" as (????) "((%&%)&H)". 
+     - inversion He1.
        iApply brel_pure_step_r; [by intros ?|done|]. 
+       iApply brel_value. by iIntros "$ !>".
+     - inversion He2.
        iApply brel_pure_step_later; [by intros ?|done|]. 
-       iApply brel_value.
-       by iIntros "!> $ !>".
-   Qed.  *)
-Admitted. 
+       iApply brel_value. by iIntros "!> !> $ !>".
+     - iApply brel_pure_step_r; [by intros ?|done|]. 
+       iApply brel_pure_step_later; [by intros ?|done|]. 
+       iApply brel_value. by iIntros "!> !> $ !>". *)
+Admitted.
 
-Lemma prel_mono `{Σ : gFunctors} e1 e2 Φ Ψ : 
+Lemma prel_mono e1 e2 Φ Ψ : 
   (∀ v1 v2, Φ v1 v2 -∗ Ψ v1 v2) -∗
-  PREL e1 ≤ e2 [{ v1; v2, Φ v1 v2}] -∗ @prel Σ e1 e2 Ψ.
+  PREL e1 ≤ e2 [{ v1; v2, Φ v1 v2}] -∗ prel e1 e2 Ψ.
 Proof.
-(*   iIntros "Hvv Hprel". rewrite /prel.
-     destruct (to_val e1) eqn:Heq1, (to_val e2) eqn:Heq2; [by iApply "Hvv" | | |].
-     1,2: iDestruct "Hprel" as (??) "($ & H)"; by iApply "Hvv".
-     iDestruct "Hprel" as (????) "($ & H)"; by iApply "Hvv".
-   Qed. *)
-Admitted. 
+  iIntros "Hvv Hprel". 
+  iRevert "Hvv". iRevert (e1 e2) "Hprel".
+  iApply (@prel_ind _ (λ ee, (∀ v1 v2 : val, Φ v1 v2 -∗ Ψ v1 v2) -∗ PREL ee.1 ≤ ee.2 [{v1; v2, Ψ v1 v2}])%I).
+  1: solve_proper.
+  iIntros ((e1,e2)) "!# IH //= Hvv".
+  rewrite !prel_unfold /prel_pre.
+  destruct (to_val e1) as [v1|]; destruct (to_val e2) as [v2|]; first by iApply "Hvv".
+  all : iIntros (?) "Hs"; iApply ("IH" with "[$][$]").
+Qed.
 
 
-Lemma prel_forall `{!Inhabited A} `{Σ : gFunctors} e1 e2 (Φ : A → val → val → iProp Σ) :
+(* (* pure_step is a partial function — uses pure_step_det + pmf_1_supp_eq *)
+   Lemma pure_step_eq (e : expr) e1 e2 : pure_step e e1 → pure_step e e2 → e1 = e2.
+   Admitted.
+   
+   (* the pure normal form of e is unique — induct on the first rtc;
+      values can't step (reducible_not_val), so the other rtc must match step-for-step *)
+   Lemma rtc_pure_step_val_det (e : expr) (v v' : val) :
+     rtc pure_step e v → rtc pure_step e v' → v = v'.
+   Admitted. *)
+
+Global Instance pwp_persistent Φ e1 e2 :
+  (∀ v1 v2, Persistent (Φ v1 v2)) → Persistent (PREL e1 ≤ e2 [{ v1;v2, Φ v1 v2 }]).
+Proof.
+  intros. rewrite prel_unseal.
+  apply (least_fixpoint_persistent_absorbing _); simpl; try apply _.
+  rewrite /prel_pre //=.
+  intros ?? (e1', e2'). 
+  destruct (to_val e1') as [v1|]; destruct (to_val e2') as [v2|]; first done.
+  - apply bi.forall_persistent. intros x. apply wand_persistent; [apply pure_plain|done|].
+Admitted.
+  
+
+Lemma prel_forall `{!Inhabited A} e1 e2 (Φ : A → val → val → iProp Σ) :
   (∀ x, PREL e1 ≤ e2 [{ (Φ x) }]) -∗ PREL e1 ≤ e2 [{ v1; v2, (∀ x, Φ x v1 v2) }].
 Proof. 
   iIntros "Hprel".
-  destruct (to_val e1) eqn:Heq1, (to_val e2) eqn:Heq2; rewrite /prel Heq1 Heq2/=; first done.
-  (* - set (x := @inhabitant A _). iSpecialize ("Hprel" $! x).
-       iDestruct "Hprel" as (??) "($ & H)". 
-       iIntros (x'). *)
-Admitted. 
+  iAssert (PREL e1 ≤ e2 [{ v1; v2, True }])%I with "[#]" as "Hwp".
+  { set (x := @inhabitant A _).
+    iSpecialize ("Hprel" $! x). 
+    iApply (prel_mono with "[][$Hprel]"); by iIntros (??) "_". }
+  iRevert "Hwp Hprel".
+  rewrite bi.intuitionistically_elim. iRevert (e1 e2).
+  iApply (@prel_ind _ (λ ee, (∀ x : A, PREL ee.1 ≤ ee.2 [{v1; v2, Φ x v1 v2}]) -∗ PREL ee.1 ≤ ee.2 [{v1; v2, ∀ x : A, Φ x v1 v2}])%I). 
+  1 : solve_proper.
+  iIntros ((e1, e2)) "!> IH H //=". rewrite prel_unfold /prel_pre.
+  destruct (to_val e1) as [v1|] eqn:He1; destruct (to_val e2) as [v2|] eqn:He2.
+  - iIntros (?). iSpecialize ("H" $! x). by rewrite prel_unfold /prel_pre He1 He2.
+  - iIntros (e2' He2'). apply of_to_val in He1 as <-. iApply "IH"; try done.
+    iIntros (?). iSpecialize ("H" $! x). rewrite prel_unfold /prel_pre He2 //=.
+    by iApply "H".
+  - iIntros (e1' He1'). apply of_to_val in He2 as <-. iApply "IH"; try done.
+    iIntros (?). iSpecialize ("H" $! x). rewrite prel_unfold /prel_pre He1 //=.
+    by iApply "H".
+  - iIntros (e1' He1'). iApply "IH"; try done.
+    iIntros (?). iSpecialize ("H" $! x). rewrite prel_unfold /prel_pre He2 He1 //=.
+    by iApply "H".
+Qed. 
+
+End prel.
